Implemented multiplication and proved it.

Binary.v
@@ -22,11 +22,15 @@ Class Binary (en : endianness) (T : Type) := {
 
   bin_plus : T -> T -> T * overflow;
   bin_plus_correct : forall t t' tt', bin_plus t t' = (tt', false) ->
-    nat_of_bin t + nat_of_bin t' = nat_of_bin tt' ;
+    nat_of_bin tt' = nat_of_bin t + nat_of_bin t' ;
 
   bin_minus : T -> T -> T * overflow;
   bin_minus_correct : forall t t' tt', bin_minus t t' = (tt', false) ->
-    nat_of_bin tt' = nat_of_bin t - nat_of_bin t'
+    nat_of_bin tt' = nat_of_bin t - nat_of_bin t' ;
+
+  bin_mult : T -> T -> T * overflow;
+  bin_mult_correct : forall t t' tt', bin_mult t t' = (tt', false) ->
+    nat_of_bin tt' = nat_of_bin t * nat_of_bin t'
 }.
 
 Definition bit := bool.
@@ -54,34 +58,38 @@ Equations vector_append_one {A} {n : nat} (v : vector A n) (a : A) : vector A (S
 vector_append_one A ?(O) Vnil w := Vcons w Vnil ;
 vector_append_one A ?(S n) (Vcons a n x) w := Vcons a (vector_append_one x w).
 
-Equations(nocomp) bits_succ (t : nat) (c : bits t) : bits t * overflow :=
+Definition zero {n} : bits n := constant_vector n false.
+Definition one {n} : bits (S n) := vector_append_one (constant_vector n false) true.
+Definition full {n} : bits n := constant_vector n true.
+
+Equations(nocomp) bits_succ {t} (c : bits t) : bits t * overflow :=
 bits_succ O v := (v, true) ;
-bits_succ (S n) (Vcons true n v) := let (v', rest) := bits_succ n v in
+bits_succ (S n) (Vcons true n v) := let (v', rest) := bits_succ v in
   (Vcons false v', rest) ;
 bits_succ (S n) (Vcons false n v) := (Vcons true v, false).
 
-Equations(nocomp) bits_succ_be (t : nat) (c : bits t) : bits t * overflow :=
+Equations(nocomp) bits_succ_be {t} (c : bits t) : bits t * overflow :=
 bits_succ_be O v := (v, true) ;
-bits_succ_be (S n) (Vcons true n v) := let (v', rest) := bits_succ_be n v in
+bits_succ_be (S n) (Vcons true n v) := let (v', rest) := bits_succ_be v in
   (Vcons true v', rest) ;
-bits_succ_be (S n) (Vcons false n v) := let (v', rest) := bits_succ_be n v in
-  if rest then (Vcons true (constant_vector n false), false) 
+bits_succ_be (S n) (Vcons false n v) := let (v', rest) := bits_succ_be v in
+  if rest then (Vcons true zero, false) 
   else (Vcons false v', false).
 
 Hint Extern 4 => progress (unfold hide_pattern in *) : Below.
 
 Fixpoint binary_of_nat_le (t : nat) (c : nat) : option (bits t) :=
   match c with
-    | 0 => Some (constant_vector t false)
+    | 0 => Some zero
     | 1 => match t with 
              | 0 => None
-             | S n => Some (Vcons true (constant_vector n false))
+             | S n => Some (Vcons true zero)
            end
     | S m => 
       match binary_of_nat_le t m with
         | None => None
         | Some m' => 
-          let (m', overflow) := bits_succ t m' in
+          let (m', overflow) := bits_succ m' in
             if overflow then None
             else Some m'
       end
@@ -89,23 +97,23 @@ Fixpoint binary_of_nat_le (t : nat) (c : nat) : option (bits t) :=
 
 Fixpoint binary_of_nat_be (t : nat) (c : nat) : option (bits t) :=
   match c with
-    | 0 => Some (constant_vector t false)
+    | 0 => Some zero
     | 1 => match t with 
              | 0 => None
-             | S n => Some (vector_append_one (constant_vector n false) true)
+             | S n => Some (vector_append_one zero true)
            end
     | S m => 
       match binary_of_nat_be t m with
         | None => None
         | Some m' => 
-          let (m', overflow) := bits_succ_be t m' in
+          let (m', overflow) := bits_succ_be m' in
             if overflow then None
             else Some m'
       end
   end.
 
-Definition one_binary_le {n : nat} : bits n :=
-  fst (bits_succ _ (constant_vector n false)).
+Definition one_binary_le {n : nat} : bits n := 
+  fst (bits_succ zero).
     
 (*
 Equations(nostruct) binary_of_nat (t : nat) (c : nat) : option (bits t) :=
@@ -209,44 +217,44 @@ Global Transparent nat_of_binary_be nat_of_binary_le.
 
 Eval compute in (nat_of_binary_be (representation 3 7)).
 
-Lemma bits_succ_be_overflow (t : nat) (b : bits t) (c : bits t) : bits_succ_be t b = (c, true) ->
-  b = c /\ b = constant_vector t true.
+Lemma bits_succ_be_overflow (t : nat) (b : bits t) (c : bits t) : bits_succ_be b = (c, true) ->
+  b = c /\ b = full.
 Proof with auto with *.
-  intros. Opaque bits_succ_be. funind (bits_succ_be t b) indbits.
+  intros. Opaque bits_succ_be. funind (bits_succ_be b) indbits.
 
     now depelim c.
 
     destruct recres. destruct o... simpdep.
     simp bits_succ_be in indbits. 
-    destruct_call bits_succ_be. destruct o ; simpdep... intuition (repeat subst ; auto).
+    destruct_call @bits_succ_be. destruct o ; simpdep... intuition (repeat subst ; auto).
 
     destruct recres. destruct o...
 Qed.
 
-Lemma nat_of_binary_bits_succ_be (t : nat) (b : bits t) (c : bits t) : bits_succ_be t b = (c, false) -> 
+Lemma nat_of_binary_bits_succ_be (t : nat) (b : bits t) (c : bits t) : bits_succ_be b = (c, false) -> 
   nat_of_binary_be c = S (nat_of_binary_be b).
 Proof with auto with *.
   intros.
   Opaque bits_succ_be binary_of_nat_be nat_of_binary_be.
-  funind (bits_succ_be t b) indbits.
+  funind (bits_succ_be b) indbits.
      
   destruct recres. program_simpl.
-  simp bits_succ_be in indbits. case_eq (bits_succ_be n v); intros.
+  simp bits_succ_be in indbits. case_eq (bits_succ_be v); intros.
   rewrite H in *. simpdep.
   Transparent nat_of_binary_be. simpl.
   rewrite IHbits_succ_be_ind. ring.
 
   destruct recres. simp bits_succ_be in indbits.
-  case_eq (bits_succ_be n v) ; intros. rewrite H in *. 
+  case_eq (bits_succ_be v) ; intros. rewrite H in *. 
   case_eq o0; case_eq o; simpdep.
   apply bits_succ_be_overflow in H. program_simpl. 
-  clear. induction n... simpl. rewrite plus_assoc, plus_0_r, <- plus_assoc. rewrite IHn.
-  ring.
+  clear. induction n... simpl. rewrite plus_assoc, plus_0_r, <- plus_assoc. 
+  unfold zero in IHn. rewrite IHn. unfold full. ring.
 
   simpl. assumption.
 Qed.
 
-Lemma binary_of_nat_be_n_O n : binary_of_nat_be (S n) 0 = Some (constant_vector (S n) false).
+Lemma binary_of_nat_be_n_O n : binary_of_nat_be (S n) 0 = Some zero.
 Proof with auto with *.
   induction n ; intros...
 Qed.
@@ -265,7 +273,7 @@ Proof with auto with *. intros n t b Htb. generalize dependent t. induction n ; 
   rewrite Hb'Sn in Htb.
   specialize (IHn _ _ Hb'Sn).
 
-  case_eq (bits_succ_be t b'); intros sb bo Hsb.
+  case_eq (bits_succ_be b'); intros sb bo Hsb.
   rewrite Hsb in *. destruct bo... program_simpl.
   now apply nat_of_binary_bits_succ_be in Hsb.
 
@@ -292,7 +300,7 @@ vfold_right2 A B C f e ?(O) Vnil Vnil := e ;
 vfold_right2 A B C f e ?(S n) (Vcons hdv n tlv) (Vcons hdv' n tlv') := 
   f n hdv hdv' (vfold_right2 f e tlv tlv').
 
-Definition bits_plus_be {n} (x y : bits n) : bits n * overflow :=
+Definition binary_plus_be {n} (x y : bits n) : bits n * overflow :=
   vfold_right2 (A:=fun n => (bits n * overflow)%type) (fun n b b' r => 
     let '(rest, carry) := r in
     let '(b, carry) := 
@@ -307,7 +315,7 @@ Definition bits_plus_be {n} (x y : bits n) : bits n * overflow :=
 Instance: Have (pow_of_2 (S n) > 0).
 Proof. reduce_goal. simp pow_of_2. induction n ; simpl ; omega. Qed.
 
-Lemma bits_plus_be_correct_full n : forall (t t' : bits n) tt' o, bits_plus_be t t' = (tt', o) ->
+Lemma binary_plus_be_correct_full n : forall (t t' : bits n) tt' o, binary_plus_be t t' = (tt', o) ->
   let add' := nat_of_binary_be t + nat_of_binary_be t' in
     if o then add' >= pow_of_2 n /\ nat_of_binary_be tt' = add' - pow_of_2 n
     else nat_of_binary_be tt' = add'.
@@ -315,10 +323,10 @@ Proof.
   intros. revert o H. induction t ; intros ; depelim t' ; try depelim tt'. simpl in *. reflexivity.
 
   destruct o.
-  unfold bits_plus_be in H.
+  unfold binary_plus_be in H.
   simp vfold_right2 in H.
-  case_eq (bits_plus_be t t'). intros. specialize (IHt _ _ _ H0).
-  unfold bits_plus_be in H0. unfold bit in * ; rewrite H0 in H.
+  case_eq (binary_plus_be t t'). intros. specialize (IHt _ _ _ H0).
+  unfold binary_plus_be in H0. unfold bit in * ; rewrite H0 in H.
   clear H0.
   
   destruct a. destruct a0 ; noconf H ; program_simpl.
@@ -336,24 +344,24 @@ Proof.
   subst add'. omega.
 
   subst add'.
-  unfold bits_plus_be in H. simp vfold_right2 in H.
-  case_eq (bits_plus_be t t'). intros. specialize (IHt _ _ _ H0).
-  unfold bits_plus_be in H0. unfold bit in * ; rewrite H0 in H.
+  unfold binary_plus_be in H. simp vfold_right2 in H.
+  case_eq (binary_plus_be t t'). intros. specialize (IHt _ _ _ H0).
+  unfold binary_plus_be in H0. unfold bit in * ; rewrite H0 in H.
   clear H0.
   destruct a ; destruct a0 ; simpl in * ; noconf H ; simpl ; try rewrite IHt ; try omega.
   destruct a1. program_simpl. rewrite H0. omega.
   assumption.
 Qed.
 
-Lemma bits_plus_be_correct n : forall (t t' : bits n) tt', bits_plus_be t t' = (tt', false) ->
+Lemma binary_plus_be_correct n : forall (t t' : bits n) tt', binary_plus_be t t' = (tt', false) ->
   nat_of_binary_be tt' = nat_of_binary_be t + nat_of_binary_be t'.
 Proof.
-  intros. apply (bits_plus_be_correct_full _ _ _ _ _ H).
+  intros. apply (binary_plus_be_correct_full _ _ _ _ _ H).
 Qed.
 
 Inductive bits_nat_view {n} : bits n -> Prop :=
 | b0 : bits_nat_view (constant_vector n false)
-| bS : forall b, bits_nat_view b -> forall b', bits_succ_be n b = (b', false) -> bits_nat_view b'.
+| bS : forall b, bits_nat_view b -> forall b', bits_succ_be b = (b', false) -> bits_nat_view b'.
 
 Print vector_ind.
 
@@ -390,10 +398,9 @@ Proof.
   simp vector_append_one.
 Qed.
 
-
 Lemma bits_succ_vector_append_0 : Π (n : nat) (v : vector bit n),
-   bits_succ_be (S n) (vector_append_one v 0%bin) =
-   (vector_append_one v 1%bin, 0%bin).
+  bits_succ_be (vector_append_one v 0%bin) =
+  (vector_append_one v 1%bin, 0%bin).
 Proof. intros.
   Opaque vector_append_one.
   funind (vector_append_one v false) appv.
@@ -444,47 +451,43 @@ binary_minus_be (S n) (Vcons hdx n tlx) (Vcons hdy n tly) :=
       (* diff (b(n-1) * 2^n-1 + ... + b0) (2^n + b'(n-1) 2^n-1 + ... + b'0) =
          ((2^n - 1) - (b(n-1) * 2^n-1 + ... + b0)) + 1 + b'(n-1) 2^n-1 + ... + b'0) *)
       let min' := Bneg _ tlx in
-      let '(plus, overflow) := bits_succ_be _ min' in
+      let '(plus, overflow) := bits_succ_be min' in
         if overflow then (* tlx must have been 0 *)
           (1 |:| tly, 1)
         else
-          let '(plus', overflow') := bits_plus_be plus tly in
+          let '(plus', overflow') := binary_plus_be plus tly in
             ((overflow' |:| plus'), 1)
     | 1, 0 => 
      (* (2^n + b(n-1) * 2^n-1 + ... + b0) - (b'(n-1) 2^n-1 + ... + b'0) =
         (2^n - 1) - (b'(n-1) 2^(n-1) + ... + b'0) + 1 + (bn * 2^(n-1) + ... + b0) *)
       let rest := Bneg _ tly in
-      let '(plus, overflow) := bits_succ_be _ rest in
+      let '(plus, overflow) := bits_succ_be rest in
         if overflow then (* tly was all zeros *)
           (1 |:| tlx, 0)
         else
-          let '(plus', overflow') := bits_plus_be plus tlx in
+          let '(plus', overflow') := binary_plus_be plus tlx in
             (overflow' |:| plus', 0)
   end.
 
 Notation " 'convertible' x y " := ((@eq_refl _ x) : x = y) (at level 0, x at next level, y at next level).
 
-Global Transparent binary_minus_be bits_plus_be bits_succ_be constant_vector vfold_right2 vector_append_one.
+Global Transparent binary_minus_be binary_plus_be bits_succ_be constant_vector vfold_right2 vector_append_one.
 
 Check (convertible (fst (binary_minus_be ninety fourty_five)) fourty_five).
 Check (convertible (nat_of_binary_be (fst (binary_minus_be fourty_five ninety))) 45).
-
-Definition zero {n} : bits n := constant_vector n false.
-Definition one {n} : bits (S n) := vector_append_one (constant_vector n false) true.
-Definition full {n} : bits n := constant_vector n true.
 
 Eval compute in (binary_minus_be (one (n:=4)) zero). 
 Eval compute in (nat_of_binary_be (fst (binary_minus_be (one (n:=4)) (representation _ 5)))).
 Eval compute in (nat_of_binary_be (fst (binary_minus_be (representation 5 5) (representation _ 5)))).
 Eval compute in (binary_minus_be (representation 5 5) (representation _ 5)).
 
-Lemma bits_succ_be_ne n y b' : bits_succ_be n (Bneg n y) = (b', 1) -> y = zero.
+Lemma bits_succ_be_ne n y b' : bits_succ_be (Bneg n y) = (b', 1) -> y = zero.
 Proof.
   induction n; intros. depelim y. reflexivity.
   
   Opaque bits_succ_be.
   depelim y.
-  case_eq (bits_succ_be n (Bneg n y)). intros. destruct o. specialize (IHn _ _ H).
+  case_eq (bits_succ_be (Bneg n y)). intros. destruct o. specialize (IHn _ _ H).
   destruct a; simp bits_succ_be in x; rewrite H in x ; noconf x. 
   subst y. reflexivity.
   
@@ -561,13 +564,13 @@ Proof.
   simpl. rewrite <- IHn. omega.
   
   clear IHn.
-  case_eq (bits_succ_be n (Bneg n y)); intros ; rewrite H0 in *.
+  case_eq (bits_succ_be (Bneg n y)); intros ; rewrite H0 in *.
   destruct o.
   noconf H. simpl. apply bits_succ_be_ne in H0. subst y. rewrite nat_of_binary_zero.
   omega.
 
-  case_eq (bits_plus_be b x); intros ; rewrite H1 in *.
-  noconf H. apply bits_plus_be_correct_full in H1. 
+  case_eq (binary_plus_be b x); intros ; rewrite H1 in *.
+  noconf H. apply binary_plus_be_correct_full in H1. 
   apply nat_of_binary_bits_succ_be in H0.
   simpl. rewrite H0 in H1. rewrite nat_of_binary_bneg in *.
   pose (nat_of_binary_bound x). 
@@ -582,8 +585,8 @@ Proof.
   replace (S (pow_of_2 n - S (nat_of_binary_be y))) with (pow_of_2 n - nat_of_binary_be y) by omega.
   omega.
 
-  destruct_call bits_succ_be. destruct o ; simpl in H. discriminate.
-  destruct_call @bits_plus_be. discriminate.
+  destruct_call @bits_succ_be. destruct o ; simpl in H. discriminate.
+  destruct_call @binary_plus_be. discriminate.
 
   case_eq (binary_minus_be x y) ; intros. rewrite H0 in *.
   noconf H.
@@ -601,7 +604,7 @@ Proof.
   depelim t ; depelim b.
   fold bit in H. unfold one in H. simp binary_minus_be in H.
   destruct a. destruct_call @bits_succ_be. destruct o. discriminate.
-  destruct_call @bits_plus_be. discriminate.
+  destruct_call @binary_plus_be. discriminate.
   case_eq (binary_minus_be t (vector_append_one (constant_vector n 0) 1)).
   intros.
   rewrite H0 in H.
@@ -641,6 +644,7 @@ Proof.
   intros n t. remember (nat_of_binary_be t) as tmp. revert n t Heqtmp. induction tmp ; intros. simpl.
   destruct n. now depelim t.
 
+  unfold zero in *. 
   funind (nat_of_binary_be t) foo. subst rest.
   destruct a. generalize (pow_of_2_pos n). intros. elimtype False. omega. 
   depind v. reflexivity. simpl. f_equal. f_equal. 
@@ -665,7 +669,7 @@ Proof.
 
   rewrite H in IHtmp.
   rewrite IHtmp.
-  case_eq (bits_succ_be (S n) b).
+  case_eq (bits_succ_be b).
   intros.
   destruct o.
   destruct (bits_succ_be_overflow _ _ _ H0). 
@@ -681,7 +685,26 @@ Proof.
   apply nat_of_binary_bits_succ_be in H0.
   rewrite Heqtmp in H0. apply nat_of_binary_be_inj in H0. congruence.
 Qed.
-  
+
+(* Inductive Split {X : Type}{m n : nat} : vector X (m + n) -> Type := *)
+(*   append : Π (xs : vector X m)(ys : vector X n), Split (vector_append xs ys). *)
+
+(* Implicit Arguments Split [ [X] ]. *)
+
+(* Equations(nocomp) split {X : Type} {m n} (xs : vector X (m + n)) : Split m n xs := *)
+(* split X O    n xs := append Vnil xs ; *)
+(* split X (S m) n (Vcons x ?(S m + n) xs) := *)
+(*   let res := split xs in *)
+(*   let 'append xs' ys' in Split _ _ vec := res return Split (S m) n (Vcons x vec) in *)
+(*     append (Vcons x xs') ys'. *)
+
+(* Equations(nocomp) split {X : Type} {m} (xs : vector X m) n : vector  *)
+(* split X O    n xs := append Vnil xs ; *)
+(* split X (S m) n (Vcons x ?(S m + n) xs) := *)
+(*   let res := split xs in *)
+(*   let 'append xs' ys' in Split _ _ vec := res return Split (S m) n (Vcons x vec) in *)
+(*     append (Vcons x xs') ys'. *)
+
 (** Binary equality *)
 
 Equations(nocomp) binary_eq {n} (x y : bits n) : bool :=
@@ -710,7 +733,170 @@ intros n. red. intros. case_eq (binary_eq x y) ; [ left | right ].
   rewrite bool_eq_refl, binary_eq_refl in foo.
   simpl in foo. discriminate.
 Qed.
-  
+
+Equations(nocomp) binary_shiftl {n} (t : bits n) : bits n * overflow :=
+binary_shiftl O Vnil := (Vnil, false) ;
+binary_shiftl (S n) (Vcons a n v) := 
+  let '(v', overflow) := binary_shiftl v in
+    (Vcons overflow v', a).
+
+Equations(nocomp) binary_shiftl_n {n} (t : bits n) (m : nat) : bits n * overflow :=
+binary_shiftl_n n t O := (t, false) ;
+binary_shiftl_n n t (S m) <= binary_shiftl t => {
+  binary_shiftl_n n t (S m) (pair t' true) := (t', true) ;
+  binary_shiftl_n n t (S m) (pair t' false) := binary_shiftl_n t' m }.
+    
+Equations(nocomp) binary_mult_be {n m} (x : bits m) (y : bits n) : bits n * overflow :=
+binary_mult_be n O Vnil y := (zero, false) ;
+binary_mult_be n (S m) (Vcons hdx m tlx) y :=
+  if hdx then 
+    let '(y', overflow) := binary_shiftl_n y m in
+      if overflow then (y, true)
+      else 
+        let '(y'', overflow) := binary_mult_be tlx y in
+          if overflow then (y, true)
+          else binary_plus_be y' y''
+  else binary_mult_be tlx y.
+
+(* Lemma binary_mult_be_0 {n} (y : bits n) z is_zero :  *)
+(*   binary_mult_be zero y true = (zero, false). *)
+(*   nat_of_binary_be x * nat_of_binary_be y = nat_of_binary_be z. *)
+(* Proof. *)
+(*   intros n m x y z is_zero. *)
+(*   funind (binary_mult_be x y is_zero) multxy. *)
+(*   simpdep. simpl. destruct is_zero. simpl. *)
+(*   intros.  *)
+
+Global Transparent binary_shiftl binary_shiftl_n binary_mult_be nat_of_binary_be.
+
+Eval compute in (binary_shiftl (one (n:=4))).
+Eval compute in (binary_shiftl (fst (binary_shiftl (one (n:=4))))).
+Eval compute in (binary_shiftl (fst (binary_shiftl (one (n:=1))))).
+Eval compute in (binary_shiftl_n (one (n:=4)) 0).
+Eval compute in (binary_shiftl_n (one (n:=4)) 4).
+Eval compute in (binary_shiftl_n (one (n:=4)) 5).
+
+Eval compute in (binary_mult_be (one (n:=4)) (one (n:=4))).
+Eval compute in (binary_mult_be (one (n:=3)) (representation 4 3)).
+Eval compute in (binary_mult_be (representation 4 2) (representation 4 3)).
+Eval compute in (nat_of_binary_be (fst (binary_mult_be (representation 4 2) (representation 4 3)))).
+Eval compute in (nat_of_binary_be (fst (binary_mult_be (representation 10 16) (representation 10 2)))).
+Eval compute in (nat_of_binary_be (fst (binary_mult_be (representation 10 16) (representation 10 0)))).
+Eval compute in (nat_of_binary_be (fst (binary_mult_be (representation 10 0) (representation 10 4)))).
+Eval compute in (nat_of_binary_be (fst (binary_mult_be (representation 10 0) (representation 10 4)))).
+Eval compute in (nat_of_binary_be (fst (binary_mult_be (representation 10 1) (representation 10 4)))).
+Eval compute in (nat_of_binary_be (fst (binary_mult_be (representation 10 2) (representation 10 4)))).
+Eval compute in (nat_of_binary_be (fst (binary_mult_be (representation 10 2) (representation 10 4)))).
+Eval compute in (nat_of_binary_be (fst (binary_mult_be (representation 10 3) (representation 10 3)))).
+
+Transparent nat_of_binary_be.
+
+Ltac case_eq_rew :=
+  fun x => generalize (@eq_refl _ x); pattern x at - 1 in |- *; case x ; intros ; 
+    on_last_hyp ltac:(fun H => rewrite H in *).
+
+
+Tactic Notation "funind" constr(c) ident(Hcall) :=
+  match c with
+    appcontext C [ ?f ] => 
+      let x := constr:(fun_ind_prf (f:=f)) in
+        (let prf := eval simpl in x in
+         let p := context C [ prf ] in
+         let prf := fresh in
+         let call := fresh in
+           assert(prf:=p) ;
+           (* Abstract the call *)
+           set(call:=c) in *; generalize (refl_equal : call = c); clearbody call ; intro Hcall ;
+           (* Now do dependent elimination and simplifications *)
+           dependent induction prf ; simplify_IH_hyps ;
+           (* Use the simplifiers for the constant to get a nicer goal. *)
+           try simpc f ; try on_last_hyp ltac:(fun id => simpc f in id ; noconf id))
+        || fail 1 "Internal error in funind"
+  end || fail "Maybe you didn't declare the functional induction principle for" c.
+
+Tactic Notation "funind" constr(c) ident(Hcall) "generalizing" ne_hyp_list(l) := 
+  match c with
+    appcontext C [ ?f ] => 
+      let x := constr:(fun_ind_prf (f:=f)) in
+        (let prf := eval simpl in x in
+         let p := context C [ prf ] in
+         let prf := fresh in
+         let call := fresh in
+           assert(prf:=p) ;
+           (* Abstract the call *)
+             set(call:=c) in *; generalize (refl_equal : call = c); intro Hcall ; revert Hcall ; clearbody call ; (* ; *)
+           (* (* Now do dependent elimination and simplifications *) *)
+           revert l ; do_depelim' ltac:(fun hyp => do_ind hyp) prf ; simplify_dep_elim ; 
+           intros ; simplify_IH_hyps ;
+           (* Use the simplifiers for the constant to get a nicer goal. *)
+           try simpc f ; try simpc f in Hcall)
+  end.
+
+Opaque binary_shiftl.
+Print Ltac funind.
+Lemma binary_shiftl_correct {n} (t : bits n) t' o : binary_shiftl t = (t', o) ->
+  if o then pow_of_2 n + nat_of_binary_be t' = 2 * nat_of_binary_be t
+  else nat_of_binary_be t' = 2 * nat_of_binary_be t.
+Proof. intros. 
+  info funind (binary_shiftl t) shiftt generalizing t' o H. 
+  destruct recres. noconf H. 
+  case_eq_rew (binary_shiftl v). noconf shiftt. 
+  destruct o. simpl. destruct o1. omega. omega. 
+  destruct o1; simpl. omega. omega.
+Qed.
+
+Transparent binary_shiftl.
+
+Lemma binary_shiftl_n_correct {n} (t : bits n) m t' : binary_shiftl_n t m = (t', false) ->
+  nat_of_binary_be t' = pow_of_2 m * nat_of_binary_be t.
+Proof. intros n t m ; revert n t ; induction m ; intros.
+
+    simp binary_shiftl_n in H. noconf H.
+
+    simp binary_shiftl_n in H. 
+    case_eq_rew (binary_shiftl t). destruct o. noconf H. 
+    specialize (IHm _ _ _ H). rewrite IHm.
+    rewrite (binary_shiftl_correct _ _ _ H0).
+    rewrite mult_assoc at 1. setoid_rewrite mult_comm at 2. simpl.
+    reflexivity.
+Qed.
+
+Lemma binary_eq_eq {n} {x y : bits n} : binary_eq x y = true -> x = y.
+Proof.
+  intros. funind (binary_eq x y) eqxy. destruct recres.
+  simp binary_eq in eqxy. rewrite andb_b_true in x. rewrite x in *.
+  simpl in *. rewrite eqxy in IHbinary_eq_ind. apply bool_eq_ok in x. subst.
+  rewrite IHbinary_eq_ind by auto. reflexivity.
+
+  rewrite andb_b_false in x. discriminate.
+Qed.
+
+Transparent binary_eq.
+Opaque binary_mult_be.
+Lemma binary_mult_correct {n m} (x : bits m) (y : bits n) z : 
+  binary_mult_be x y = (z, false) -> nat_of_binary_be x * nat_of_binary_be y = nat_of_binary_be z.
+Proof.
+  intros n m x. induction x ; intros.
+  simp binary_mult_be in H. noconf H.
+  rewrite nat_of_binary_zero. reflexivity. 
+
+  simp binary_mult_be in H.
+  destruct a. 
+  case_eq (binary_shiftl_n y n0) ; intros. rewrite H0 in *.
+  case_eq_rew (binary_mult_be x y). 
+  destruct o ; try noconf H.
+  destruct o0. noconf H.
+  specialize (IHx _ _ H1).
+  apply binary_shiftl_n_correct in H0.
+  apply binary_plus_be_correct in H.
+  rewrite H.
+  rewrite <- IHx. rewrite H0. ring.
+
+  specialize (IHx _ _ H).
+  assumption.
+Qed.
+Transparent binary_mult_be.
+
 Definition coerce_bits {n m} (c : bits n) (H : n = m) : bits m.
 Proof. intros ; subst. exact c. Defined.
 
@@ -732,17 +918,19 @@ Program Instance bvec_binary_be n : Binary BigEndian (bits (S n)) := {
   bin_of_nat := binary_of_nat_be (S n);
   nat_of_bin := nat_of_binary_be;
 
-  bin_succ := bits_succ_be (S n) ;
+  bin_succ := bits_succ_be ;
 
-  bin_plus := bits_plus_be ;
-  bin_minus := binary_minus_be 
+  bin_plus := binary_plus_be ;
+  bin_minus := binary_minus_be ;
+  bin_mult := binary_mult_be
 }.
 
   Next Obligation. now apply nat_of_binary_inverse. Qed.
   Next Obligation. apply binary_of_nat_inverse. Qed.
   Next Obligation. now erewrite nat_of_binary_bits_succ_be. Qed.
-  Next Obligation. symmetry. now apply bits_plus_be_correct. Qed.
+  Next Obligation. now apply binary_plus_be_correct. Qed.
   Next Obligation. symmetry. now apply binary_minus_correct. Qed.
+  Next Obligation. symmetry. now apply binary_mult_correct. Qed.
 
 Global Transparent vfold_right2 binary_minus_be bits_succ_be nat_of_binary_be.
 
@@ -752,3 +940,40 @@ Eval compute in (nat_of_bin (fst (bin_plus fourty_five ninety))).
 
 Eval compute in (nat_of_bin (fst (bin_minus fourty_five ninety))).
 Eval compute in (nat_of_bin (fst (bin_minus ninety fourty_five))).
+
+
+(** Orders *)
+
+Equations(nocomp) binary_be_le {n} (x y : bits n) : bool :=
+binary_be_le O Vnil Vnil := true ;
+binary_be_le (S n) (Vcons a n x) (Vcons a' n y) :=
+  if xorb a a' then a'
+  else binary_be_le x y.
+
+Class BoolReflexive {A} (R : A -> A -> bool) := 
+  reflexivityb : forall x, R x x = true.
+
+Class BoolSymmetric {A} (R : A -> A -> bool) := 
+  symmetryb : forall x y, R x y = true -> R y x = true.
+
+Class BoolTransitive {A} (R : A -> A -> bool) := 
+  transitivityb : forall x y z, R x y = true -> R y z = true -> R x z = true.
+
+Instance: BoolReflexive (@binary_be_le n).
+Proof. reduce_goal. induction x ; simp binary_be_le.
+  rewrite IHx. destruct a ; simpl ; auto.
+Qed.
+
+Instance: BoolTransitive (@binary_be_le n).
+Proof. reduce_goal. induction x ; simp binary_be_le; depelim y ; depelim z.
+  simp binary_be_le.
+
+  simp binary_be_le in H.
+  simp binary_be_le in H0. 
+  destruct a ; destruct a1 ; destruct a0 ; simpl in * ; try discriminate ; simp binary_be_le.
+Qed.
+
+Definition binary_le_lt {n} (x y : bits n) := 
+  let '(x', overflow) := bits_succ_be x in
+    if overflow then false
+    else binary_be_le x' y.
